Define 'blocked_trim_quad1'
Also, prove the conditions under which a trace will remain unchanged
when applying this filter to its blocked list. Note that this is the
filter which will be used to create the final blocked list, with
'top' set to match the y-coordinate of the top cell in the west wall.

AngelDevil/Blocked.lean
@@ -326,3 +326,72 @@ lemma trace_trim_neg_one_unchanged (n : Nat) (start : RunState) (blocked : List 
       have hleft' : loc (turn_left rs) ∉ blocked' :=
         fun h ↦ False.elim (hleft (hss h))
       rw [if_neg hleft, if_neg hleft']
+
+-- I tried getting List.max? to work, but it was more effort than just writing
+-- out the 18 lines of code below
+def list_int_max (L : List Int) : Int :=
+  match L with
+  | []      => 0
+  | x :: xs => max x (list_int_max xs)
+
+lemma list_int_max_cons (a : Int) (L : List Int) :
+  list_int_max (a :: L) = max a (list_int_max L) := rfl
+
+lemma list_int_le_max (L : List Int) :
+  ∀ a ∈ L, a ≤ list_int_max L :=
+  match L with
+  | []      => fun _ amem ↦ False.elim (List.not_mem_nil amem)
+  | x :: xs => by
+    intro a amem
+    rw [list_int_max_cons]
+    rcases List.mem_cons.mp amem with rfl | rhs
+    · exact Int.le_max_left _ _
+    · exact le_max_of_le_right (list_int_le_max xs a rhs)
+
+-- Blocked list filter that only keeps cells with -1 ≤ x, 0 ≤ y, y ≤ top, and
+-- x-coordinate less than or equal to one more than the maximum x coordinate in the trace
+-- To construct the final blocked list, this filter will be used with 'top' chosen
+-- to match the height of the west wall.
+def blocked_trim_quad1
+  (n : Nat) (start : RunState) (blocked : List (Int × Int)) (top : Int) : List (Int × Int) :=
+  blocked_trim_neg_one (blocked_trim_rect top (-1) (-1)
+    (list_int_max (List.map (fun a ↦ a.x) (trace n start blocked)) + 1) blocked)
+
+-- Prove the conditions under which the trace is unchanged by 'blocked_trim_quad1'
+lemma trace_trim_quad1_unchanged
+  (n : Nat) (start : RunState) (blocked : List (Int × Int)) (top : Int) :
+  (∀ rs ∈ trace n start blocked,
+  0 ≤ rs.x ∧ 0 ≤ rs.y ∧ rs.y < top ∧ (rs.y = 0 → rs.u ≠ uvec_left)) →
+  trace n start blocked = trace n start (blocked_trim_quad1 n start blocked top) := by
+  intro h
+  -- Prove that the bounds for the rectangular filter follow from the givens
+  have hbounds : ∀ (i : ℕ) (ilt : i < n),
+    (fun a ↦ a.y < top ∧ -1 < a.y ∧ -1 < a.x ∧
+     a.x < list_int_max (List.map (fun a ↦ a.x) (trace n start blocked)) + 1)
+    ((trace n start blocked)[i]'(by rwa [trace_length])) := by
+    intro i ilt
+    constructor
+    · exact (h _ (List.getElem_mem _)).2.2.1
+    constructor
+    · apply Int.lt_of_sub_pos; simp
+      apply Int.lt_add_one_of_le
+      exact (h _ (List.getElem_mem _)).2.1
+    constructor
+    · apply Int.lt_of_sub_pos; simp
+      apply Int.lt_add_one_of_le
+      exact (h _ (List.getElem_mem _)).1
+    · apply Int.lt_add_one_of_le
+      apply list_int_le_max
+      apply List.mem_map.mpr
+      exact ⟨_, List.getElem_mem _, rfl⟩
+  unfold blocked_trim_quad1
+  rw [← trace_trim_neg_one_unchanged]
+  · rwa [← trace_trim_rect_unchanged]
+  intro i ilt
+  -- Reorder / repackage the bounds for the y = -1 filter
+  have h' : ∀ rs ∈ trace n start blocked, 0 ≤ rs.y ∧ (rs.y = 0 → rs.u ≠ uvec_left) :=
+    fun rs rsmem ↦ ⟨(h rs rsmem).2.1, (h rs rsmem).2.2.2⟩
+  apply h'
+  convert List.getElem_mem _ using 2; swap
+  · rwa [trace_length]
+  rwa [← trace_trim_rect_unchanged]
